\newcommand\phidash[1]{\ensuremath{\phi\ '(#1)}}
\newcommand\phif[1]{\ensuremath{\phi\ (#1)}}
\newcommand\amcost{\ensuremath{\hat{c}_i}}
\newcommand\accost{\ensuremath{c_i}}

Let

\begin{displaymath}
\phidash{D_i} = \phif{D_i} - \phif{D_0}
\end{displaymath}

then
\begin{eqnarray*}
\phidash{D_0} &=& 0 \\
\phidash{D_i} &\geq& 0 \ (\because\ \phif{D_i} \geq\ \phif{D_0})
\end{eqnarray*}

Now the amortized cost using \phidash{D} is,

\begin{eqnarray*}
\sum_{i=1}^{n} \amcost &=& \sum_{i=1}^{n} \accost + \phidash{D_n} -
\phidash{D_0} \\
&=& \sum_{i=1}^{n} \accost + \phif{D_n} - \phif{D_0} - 
( \phif{D_0} - \phif{D_0}) \\
&=& \sum_{i=1}^{n} \accost + \phif{D_n} - \phif{D_0}
\end{eqnarray*}

which is same as the amortized cost using \phif{D}.
